aux_fun_tests.v
@@ -242,6 +242,204 @@ Ltac kooooo t na :=
    constr:((4,5)).
 
 
+   Inductive my_idents :=
+   | one_id {A : Type} (a : A) : my_idents.
+
+(* Temporary: obtaining tVar list*)
+
+(* Section  Clearbod.
+
+
+From Ltac2 Require Ltac2.
+From Coq Require Import Strings.String.
+From Coq Require Import Init.Byte.
+
+
+Import List.ListNotations.
+Local Open Scope list.
+
+Import Ltac2.
+
+
+Ltac2 Type exn ::= [ NotStringLiteral(constr) | InvalidIdent(string) ].
+
+Ltac2 coq_byte_to_int b :=
+    (match! b with
+     (* generate this line with python3 -c 'print(" ".join([\'| x%02x => %d\' % (x,x) for x in range(256)]))' *)
+     | x00 => 0 | x01 => 1 | x02 => 2 | x03 => 3 | x04 => 4 | x05 => 5 | x06 => 6 | x07 => 7 | x08 => 8 | x09 => 9 | x0a => 10 | x0b => 11 | x0c => 12 | x0d => 13 | x0e => 14 | x0f => 15 | x10 => 16 | x11 => 17 | x12 => 18 | x13 => 19 | x14 => 20 | x15 => 21 | x16 => 22 | x17 => 23 | x18 => 24 | x19 => 25 | x1a => 26 | x1b => 27 | x1c => 28 | x1d => 29 | x1e => 30 | x1f => 31 | x20 => 32 | x21 => 33 | x22 => 34 | x23 => 35 | x24 => 36 | x25 => 37 | x26 => 38 | x27 => 39 | x28 => 40 | x29 => 41 | x2a => 42 | x2b => 43 | x2c => 44 | x2d => 45 | x2e => 46 | x2f => 47 | x30 => 48 | x31 => 49 | x32 => 50 | x33 => 51 | x34 => 52 | x35 => 53 | x36 => 54 | x37 => 55 | x38 => 56 | x39 => 57 | x3a => 58 | x3b => 59 | x3c => 60 | x3d => 61 | x3e => 62 | x3f => 63 | x40 => 64 | x41 => 65 | x42 => 66 | x43 => 67 | x44 => 68 | x45 => 69 | x46 => 70 | x47 => 71 | x48 => 72 | x49 => 73 | x4a => 74 | x4b => 75 | x4c => 76 | x4d => 77 | x4e => 78 | x4f => 79 | x50 => 80 | x51 => 81 | x52 => 82 | x53 => 83 | x54 => 84 | x55 => 85 | x56 => 86 | x57 => 87 | x58 => 88 | x59 => 89 | x5a => 90 | x5b => 91 | x5c => 92 | x5d => 93 | x5e => 94 | x5f => 95 | x60 => 96 | x61 => 97 | x62 => 98 | x63 => 99 | x64 => 100 | x65 => 101 | x66 => 102 | x67 => 103 | x68 => 104 | x69 => 105 | x6a => 106 | x6b => 107 | x6c => 108 | x6d => 109 | x6e => 110 | x6f => 111 | x70 => 112 | x71 => 113 | x72 => 114 | x73 => 115 | x74 => 116 | x75 => 117 | x76 => 118 | x77 => 119 | x78 => 120 | x79 => 121 | x7a => 122 | x7b => 123 | x7c => 124 | x7d => 125 | x7e => 126 | x7f => 127 | x80 => 128 | x81 => 129 | x82 => 130 | x83 => 131 | x84 => 132 | x85 => 133 | x86 => 134 | x87 => 135 | x88 => 136 | x89 => 137 | x8a => 138 | x8b => 139 | x8c => 140 | x8d => 141 | x8e => 142 | x8f => 143 | x90 => 144 | x91 => 145 | x92 => 146 | x93 => 147 | x94 => 148 | x95 => 149 | x96 => 150 | x97 => 151 | x98 => 152 | x99 => 153 | x9a => 154 | x9b => 155 | x9c => 156 | x9d => 157 | x9e => 158 | x9f => 159 | xa0 => 160 | xa1 => 161 | xa2 => 162 | xa3 => 163 | xa4 => 164 | xa5 => 165 | xa6 => 166 | xa7 => 167 | xa8 => 168 | xa9 => 169 | xaa => 170 | xab => 171 | xac => 172 | xad => 173 | xae => 174 | xaf => 175 | xb0 => 176 | xb1 => 177 | xb2 => 178 | xb3 => 179 | xb4 => 180 | xb5 => 181 | xb6 => 182 | xb7 => 183 | xb8 => 184 | xb9 => 185 | xba => 186 | xbb => 187 | xbc => 188 | xbd => 189 | xbe => 190 | xbf => 191 | xc0 => 192 | xc1 => 193 | xc2 => 194 | xc3 => 195 | xc4 => 196 | xc5 => 197 | xc6 => 198 | xc7 => 199 | xc8 => 200 | xc9 => 201 | xca => 202 | xcb => 203 | xcc => 204 | xcd => 205 | xce => 206 | xcf => 207 | xd0 => 208 | xd1 => 209 | xd2 => 210 | xd3 => 211 | xd4 => 212 | xd5 => 213 | xd6 => 214 | xd7 => 215 | xd8 => 216 | xd9 => 217 | xda => 218 | xdb => 219 | xdc => 220 | xdd => 221 | xde => 222 | xdf => 223 | xe0 => 224 | xe1 => 225 | xe2 => 226 | xe3 => 227 | xe4 => 228 | xe5 => 229 | xe6 => 230 | xe7 => 231 | xe8 => 232 | xe9 => 233 | xea => 234 | xeb => 235 | xec => 236 | xed => 237 | xee => 238 | xef => 239 | xf0 => 240 | xf1 => 241 | xf2 => 242 | xf3 => 243 | xf4 => 244 | xf5 => 245 | xf6 => 246 | xf7 => 247 | xf8 => 248 | xf9 => 249 | xfa => 250 | xfb => 251 | xfc => 252 | xfd => 253 | xfe => 254 | xff => 255
+     end).
+
+
+Ltac2 coq_byte_to_char b :=
+    Char.of_int (coq_byte_to_int b).
+
+Fixpoint coq_string_to_list_byte (s : string) : list byte :=
+  match s with
+  | EmptyString => []
+  | String c s => Ascii.byte_of_ascii c :: coq_string_to_list_byte s
+   end.
+
+  (** copy a list of Coq byte constrs into a string (already of the right length) *)
+  Ltac2 rec coq_byte_list_blit_list (pos : int) (ls : constr) (str : string) :=
+    match! ls with
+    | nil => ()
+    | ?c :: ?ls =>
+      let b := coq_byte_to_char c in
+      String.set str pos b; coq_byte_list_blit_list (Int.add pos 1) ls str
+  end.
+
+  Ltac2 rec coq_string_length (s : constr) :=
+    match! s with
+    | EmptyString => 0
+    | String _ ?s' => Int.add 1 (coq_string_length s')
+    | _ => Control.throw (NotStringLiteral(s))
+    end.
+
+  Ltac2 compute c :=
+    Std.eval_vm None c.
+
+  (** [coq_string_to_string] converts a Gallina string in a constr to an Ltac2
+  native string *)
+  Ltac2 coq_string_to_string (s : constr) :=
+    let l := coq_string_length s in
+    let str := String.make l (Char.of_int 0) in
+    let bytes := compute constr:(coq_string_to_list_byte $s) in
+    let _ := coq_byte_list_blit_list 0 bytes str in
+    str.
+
+  Ltac2 ident_from_string (s : string) :=
+    match Ident.of_string s with
+    | Some id => id
+    | None => Control.throw (InvalidIdent s)
+    end.
+
+    Ltac2 coq_string_to_ident (s : constr) := ident_from_string (coq_string_to_string s).
+
+    Ltac2 get_opt o := match o with None => Control.throw Not_found | Some x => x end.
+
+ 
+
+
+(* 
+Ltac2 clearbody_id (t : constr)  :=  
+       match! t with
+       | one_id ?idn => let x := ident_from_string (coq_string_to_string idn) in  
+        ltac1:(x |- clearbody x) 
+   end. *)
+
+
+(*
+Ltac2 rec clearbody_id_list (l : constr)  :=  
+   match! l with
+  | [] => () 
+  | ?ctor :: ?l0 => match! ctor with
+    | one_id ?idn => let x := coq_string_to_string (idn) in 
+     ltac1:(x |- clearbody x) ; clearbody_id_list l0
+end
+end. *)
+Ltac2 cleabody2 s := ltac1:(s |- clearbody s).
+
+Fail Ltac clearbody_id s := ltac2:(s1 |- let s := get_opt (Ltac1.to_constr s1) in
+let ident := coq_string_to_ident s in
+clearbody2 ident).
+
+(* Ltac clearbody_id s := ltac2:(s1 |- let s2 := get_opt (Ltac1.to_constr s1) in
+let ident := coq_string_to_ident s2 in
+clearbody2 s2). *)
+
+
+Goal forall (n1 n2 : nat) (b1 b2 : bool), False.
+Proof.
+intros. 
+pose (one_id "n2") as k. 
+Fail clearbody_id k.
+pose [ one_id "n1" ; one_id "b2"] as l0.
+Fail clearbody_id_list l0.
+pose [[ one_id "n1" ; one_id "b2"] ; [] ; [one_id "b1"]] as l. 
+Fail clearbody_id_llist l.
+Abort.
+
+
+
+From Coq Require Import List.
+Import ListNotations.
+
+
+
+Ltac clearbody_id_ctor ctor :=
+  match eval hnf in ctor with
+  | one_id ?idn =>
+    clearbody idn
+  end.
+
+Ltac clearbody_id_list l :=
+  match eval hnf in l with
+  | [] => idtac
+  | ?ctor :: ?l0 =>
+    clearbody_id_ctor ctor ;
+    clearbody_id_list l0
+end.
+
+Ltac clearbody_id_llist l :=
+  match eval hnf in l with
+  | [] => idtac
+  | ?l0 :: ?tl0 => clearbody_id_list l0 ; clearbody_id_llist tl0
+end.
+
+
+Goal False.
+pose (n3 := 0). 
+Fail clearbody_id_ctor (one_id n3).
+Abort. 
+
+From Coq Require Import List.
+Import ListNotations.
+
+End Clearbod. *)
+
+
+Ltac clearbody_id_list l :=  
+  lazymatch eval hnf in l with
+  | [] => idtac 
+  | [?ctor ] => lazymatch eval hnf in ctor with 
+    | one_id ?idn => clearbody idn end   
+  | ?ctor :: ?l0 => lazymatch eval hnf in ctor with
+    | one_id ?idn => let x := constr:(idn) in 
+    let _ := match goal with _ => clearbody x end in clearbody_id_list l0
+end
+end. 
+
+
+Ltac clearbody_id_llist l :=
+  match eval hnf in l with
+  | [] => idtac
+  | ?l0 :: ?tl0 => clearbody_id_list l0 ; clearbody_id_llist tl0
+end. 
+
+
+
+Goal forall (n1 n2 : nat) (b1 b2 : bool), False.
+Proof.
+intros.
+pose [[ one_id "n1" ; one_id "b2"] ; [] ; [one_id "b1"]] as l. 
+pose [ one_id "n1" ; one_id "b2"] as l0.
+Fail clearbody_id_list l0.
+Fail clearbody_id_llist l.
+Abort.
+
+
+
+Ltac clearbody_id_ctor ctor :=
+  match eval hnf in ctor with
+  | one_id ?idn =>
+    clearbody idn
+  end.
+
+
+  Goal False.
+  pose (n3 := 0).
+ Fail clearbody_id_ctor (one_id n3).
+  Abort. 
 
 (***********************************)
 
@@ -507,7 +705,8 @@ Abort.
 
 
 Goal False.
-let x := constr:(is_inj (tApp list_reif [tRel 2]) cons_reif [tRel 0 ; tApp list_reif [tRel 1]] 1 ) in pose x as is_inj_cons ; compute in is_inj_cons.
+let x := constr:(is_inj (tApp list_reif [tRel 2]) cons_reif [Set_reif ; tRel 0 ; tApp list_reif [tRel 1]] 1) in pose x as is_inj_cons ; compute in is_inj_cons.
+pose_unquote_term_hnf is_inj_cons is_inj_cons_blut.
 Abort.
 
 
